src/lib/Basic.v
@@ -19,6 +19,9 @@ Require Import HahnRelationsBasic.
 Set Implicit Arguments.
 
 
+Axiom devil: False.
+Ltac admit := exfalso; clear; case devil.
+
 Ltac refl := reflexivity.
 Ltac congr := congruence.
 Ltac etrans := etransitivity.
@@ -898,5 +901,27 @@ Module IdSet.
   Qed.
 End IdSet.
 
-Axiom devil: False.
-Ltac admit := exfalso; clear; case devil.
+Inductive inverse A (rel:relation A) (codom:A -> Prop) (a:A): Prop :=
+| inverse_intro
+    a'
+    (REL: rel a a')
+    (CODOM: codom a')
+.
+Hint Constructors inverse.
+
+Lemma inverse_mon A (r1 r2:relation A)
+      (REL: r1 ⊆ r2):
+  inverse r1 <2= inverse r2.
+Proof.
+  i. inv PR. econs; eauto.
+Qed.
+
+Lemma inverse_union A (r1 r2:relation A) s:
+  inverse (r1 ∪ r2) s = inverse r1 s \1/ inverse r2 s.
+Proof.
+  funext. i. propext. econs; i.
+  - inv H. inv REL; eauto.
+  - des; inv H; econs; eauto.
+    + left. ss.
+    + right. ss.
+Qed.
