src/axiomatic/AtoP.v
@@ -19,7 +19,7 @@ Require Import PromisingArch.lib.Lang.
 Require Import PromisingArch.promising.Promising.
 Require Import PromisingArch.promising.CommonPromising.
 Require Import PromisingArch.axiomatic.Axiomatic.
-Require Import PromisingArch.axiomatic.CommonAxiomatic.
+Require Import PromisingArch.axiomatic.SimLocal.
 
 Set Implicit Arguments.
 
