src/axiomatic/TsoPFtoA.v
@@ -22,7 +22,7 @@ Require Import PromisingArch.promising.CommonPromising.
 Require Import PromisingArch.promising.TsoStateExecFacts.
 Require Import PromisingArch.promising.TsoPtoPF.
 Require Import PromisingArch.axiomatic.TsoAxiomatic.
-Require Import PromisingArch.axiomatic.TsoCommonAxiomatic.
+Require Import PromisingArch.axiomatic.TsoSimLocal.
 Require Import PromisingArch.axiomatic.TsoPFtoA1.
 Require Import PromisingArch.axiomatic.TsoPFtoA2.
 Require Import PromisingArch.axiomatic.TsoPFtoA3.
