src/axiomatic/TsoPFtoA1.v
@@ -20,7 +20,7 @@ Require Import PromisingArch.promising.TsoPromising.
 Require Import PromisingArch.promising.CommonPromising.
 Require Import PromisingArch.promising.TsoStateExecFacts.
 Require Import PromisingArch.axiomatic.TsoAxiomatic.
-Require Import PromisingArch.axiomatic.TsoCommonAxiomatic.
+Require Import PromisingArch.axiomatic.TsoSimLocal.
 
 Set Implicit Arguments.
 
